ott_coq/destination_calculus_sugar_typing.v
@@ -26,11 +26,11 @@ Proof.
   apply Ty_term_Val.
   - assumption.
   - rewrite union_empty_r_eq with (G := ᴳ{}).
-    assert (hvarsᴳ(ᴳ- ᴳ{+ 1 : ¹ν ⌊ T ⌋ ¹ν }) = ᴴ{ 1}) as hvarsD3Eq.
-      { rewrite hvars_minus_eq. unfold hvars_ctx, hvars_dom, ctx_singleton, hminus. rewrite dom_singleton_eq. cbn. reflexivity. }
+    assert (hvarsᴳ(ᴳ-⁻¹ ᴳ{- 1 : ¹ν ⌊ T ⌋ ¹ν }) = ᴴ{ 1}) as hvarsD3Eq.
+      { rewrite hvars_minus_eq. unfold hvars_ctx, hvars_dom, ctx_singleton, hminus_inv. rewrite dom_singleton_eq. cbn. reflexivity. }
     rewrite <- hvarsD3Eq. apply Ty_val_Ampar; swap 1 10; swap 2 11.
     + rewrite stimes_empty_eq, <- union_empty_l_eq. apply Ty_val_Dest.
-    + rewrite <- union_empty_l_eq. rewrite hminus_singleton. apply Ty_val_Hole.
+    + rewrite <- union_empty_l_eq. rewrite hminus_inv_singleton. apply Ty_val_Hole.
     + apply DestOnly_singleton_dest.
     + apply LinOnly_singleton_iff. cbn. constructor.
     + apply FinAgeOnly_singleton_iff. cbn. constructor.
